lemmes de substitution

theories/quotlambda_new.v
@@ -554,6 +554,9 @@ Proof. by rewrite /actN /= /atomact tfinpermL. Qed.
 Lemma swapR a b : (swap a b) \dot b = a.
 Proof. by rewrite /actN /= /atomact tfinpermR. Qed.
 
+Lemma atomactE π a : π \dot a = π a.
+Proof. by []. Qed.
+
 End NominalAtoms.
 
 
@@ -702,6 +705,14 @@ Proof.
 apply act_id => b bsuppx. case: tfinpermP => //= b_eq; rewrite b_eq in bsuppx. 
   by rewrite bsuppx in a_fresh_x.
 by rewrite bsuppx in a'_fresh_x.
+Qed.
+
+Lemma fresh_perm (π : finPerm) (x : X) : 
+  [disjoint (support x) & finsupp π] -> π \dot x = x.
+Proof.
+move => /fdisjointP disj_x_π.  
+apply act_id => a /disj_x_π.
+exact: finsfun_dflt.
 Qed.
 
 End Freshness.
@@ -1885,3 +1896,65 @@ admit.
 rewrite -pi_equivariant. admit.
 Qed.
 
+End EliminationPrinciples.
+
+Section Subst.
+
+
+Variables (x : atom) (t : term).
+
+Definition dflt := Var 0.
+
+Definition subst_f1 y := if x == y then t else Var y.
+Definition subst_f2 (t1 t2 : term) subst_t1 subst_t2 :=
+  App subst_t1 subst_t2.
+Definition subst_f3 x (t : term) subst_t := Lambda x subst_t.
+
+Lemma if_equivariant (X : nominalType) (b : bool) (t1 t2 : X) π :
+  (π \dot (if b then t1 else t2)) = (if b then (π \dot t1) else (π \dot t2)). 
+Proof. by case: b. Qed.
+
+Lemma support_subst_f1 : function_support1 subst_f1 (x |: support t).
+Proof.
+move=>π; rewrite fset1_disjoint => /andP [xNπ disj_t_π] y.
+have xNπinv : x \notin finsupp π^-1 by [].
+by rewrite/subst_f1 if_equivariant Var_equiv atomactE [_ == π _]eq_sym 
+finperm_can2eq eq_sym (finsfun_dflt xNπinv) (fresh_perm disj_t_π).
+Qed.
+
+Lemma support_subst_f2 : function_support4 subst_f2 fset0.
+Proof.
+move => π _ t1 t2 u1 u2. 
+by rewrite /subst_f2 App_equiv.
+Qed.
+
+Lemma support_subst_f3 : function_support3 subst_f3 fset0.
+Proof.
+move => π _ y u v.
+by rewrite /subst_f3 Lam_equiv.
+Qed.
+
+Lemma FCB_f3 : FCB subst_f3.
+Proof.
+exists (@fset0 nat_KeyType) => y u v.
+admit.
+Qed.
+
+Definition subst := term_altrect subst_f1 subst_f2 subst_f3 (x |: support t) fset0 fset0 dflt.
+
+Lemma subst_VarE y : subst (Var y) = if x == y then t else Var y. 
+Proof.
+by rewrite/subst term_altrect_VarE /subst_f1.
+Qed.
+
+Lemma subst_AppE t1 t2 : subst (App t1 t2) = App (subst t1) (subst t2).
+Proof.
+by rewrite/subst term_altrect_AppE /subst_f2.
+Qed.
+
+Lemma subst_LamE y u : subst (Lambda y u) = Lambda y (subst u).
+Proof.
+rewrite/subst term_altrect_LamE /subst_f3 //.
+  exact: support_subst_f1.
+  exact: support_subst_f2.
+  exact: support_subst_f3.
